cfrontend/Cminorgenproof.v
@@ -2309,20 +2309,20 @@ Proof.
 Qed.
 
 Lemma transl_external:
-  forall (w: ccworld cc_inject_triangle) S R q1 AE1,
+  forall (w: ccworld cc_inject_triangle) S R q1,
   match_states w S R ->
-  make_external (Csharpminor.at_external ge) Csharpminor.after_external S q1 AE1 ->
-  exists wA q2 AE2,
+  Csharpminor.at_external ge S q1 ->
+  exists wA q2,
     match_query (cc_c injp) wA q1 q2 /\
-    make_external (Cminor.at_external tge) Cminor.after_external R q2 AE2 /\
+    Cminor.at_external tge R q2 /\
     forall r1 r2 S',
       match_reply (cc_c injp) wA r1 r2 ->
-      AE1 r1 S' ->
+      Csharpminor.after_external S r1 S' ->
       exists R',
-        AE2 r2 R' /\
+        Cminor.after_external R r2 R' /\
         match_states w S' R'.
 Proof.
-  intros w S R q1 AE1 HSR Hq1. destruct Hq1 as [S q1 Hq1].
+  intros w S R q1 HSR Hq1.
   destruct Hq1 as [b id sg vargs1 k1 m1 Hb].
   inv HSR.
   edestruct (match_cc_inject b sg) as (wA & Hq & H); eauto.
@@ -2338,9 +2338,8 @@ Proof.
   }
   inv TR.
   assert (fd = External (EF_external id sg)) by congruence; subst fd.
-  eexists wA, (cq b sg targs tm), _; repeat apply conj; eauto.
+  exists wA, (cq b sg targs tm); repeat apply conj; eauto.
   - inv H1.
-    constructor.
     econstructor; eauto.
   - intros [vres1 m1'] [vres2 m2'] S' Hr HS'.
     inv HS'.
